theories/zoo_saturn/mpmc_stack_1__opaque.v
@@ -1,6 +1,0 @@
-Require Import zoo_saturn.mpmc_stack_1__code.
-
-#[global] Opaque mpmc_stack_1٠create.
-#[global] Opaque mpmc_stack_1٠push.
-#[global] Opaque mpmc_stack_1٠pop.
-#[global] Opaque mpmc_stack_1٠snapshot.
