theories/zoo_saturn/stack_mpmc_1__opaque.v
@@ -1,0 +1,6 @@
+Require Import zoo_saturn.stack_mpmc_1__code.
+
+#[global] Opaque stack_mpmc_1٠create.
+#[global] Opaque stack_mpmc_1٠push.
+#[global] Opaque stack_mpmc_1٠pop.
+#[global] Opaque stack_mpmc_1٠snapshot.
